test/Util/TestUtils.dfy
@@ -2,12 +2,12 @@
 // SPDX-License-Identifier: Apache-2.0
 
 include "../../src/SDK/Keyring/RawAESKeyring.dfy"
-include "../../src/Crypto/EncryptionSuites.dfy"
 include "../../src/StandardLibrary/StandardLibrary.dfy"
 include "../../src/StandardLibrary/UInt.dfy"
 include "../../src/Util/UTF8.dfy"
 include "../../src/SDK/Materials.dfy"
 include "../../src/SDK/EncryptionContext.dfy"
+include "../../src/Crypto/AESEncryption.dfy"
 include "../../src/SDK/MessageHeader.dfy"
 
 module {:extern "TestUtils"} TestUtils {
@@ -19,7 +19,7 @@ module {:extern "TestUtils"} TestUtils {
   import EncryptionContext
   import MessageHeader
   import RawAESKeyringDef
-  import EncryptionSuites
+  import AESEncryption
 
   const SHARED_TEST_KEY_ARN := "arn:aws:kms:us-west-2:658956600833:key/b3537ef1-d8dc-4780-9f5a-55776cbb2f7f";
 
@@ -161,7 +161,15 @@ module {:extern "TestUtils"} TestUtils {
   {
     var namespace :- UTF8.Encode("namespace");
     var name :- UTF8.Encode("MyKeyring");
-    var keyring := new RawAESKeyringDef.RawAESKeyring(namespace, name, seq(32, i => 0), EncryptionSuites.AES_GCM_256);
+    var keyring := new RawAESKeyringDef.RawAESKeyring(
+      namespace,
+      name,
+      seq(32, i => 0),
+      AESEncryption.AES_GCM(
+        keyLength := 32 as AESEncryption.KeyLength,
+        tagLength := 16 as AESEncryption.TagLength,
+        ivLength := 12 as AESEncryption.IVLength
+      ));
     return Success(keyring);
   }
 
